Logic/Modal/Standard/Complemental.lean
@@ -101,16 +101,20 @@ postfix:80 "⁻" => Formulae.complementary
 
 variable {P P₁ P₂ : Formulae α} {p q r: Formula α}
 
-lemma complementary_mem : p ∈ P → p ∈ P⁻ := by simp [complementary]; tauto;
+lemma complementary_mem (h : p ∈ P) : p ∈ P⁻ := by simp [complementary]; tauto;
+macro_rules | `(tactic| trivial) => `(tactic| apply complementary_mem $ by assumption)
 
-lemma complementary_mem_box [P.SubformulaClosed] : □p ∈ P⁻ → □p ∈ P := by
+lemma complementary_comp (h : p ∈ P) : -p ∈ P⁻ := by simp [complementary]; tauto;
+macro_rules | `(tactic| trivial) => `(tactic| apply complementary_comp $ by assumption)
+
+lemma complementary_mem_box (hi : ∀ {q r}, q ⟶ r ∈ P → q ∈ P := by trivial) : □p ∈ P⁻ → □p ∈ P := by
   simp [complementary];
   intro h;
   rcases h with (h | ⟨q, hq, eq⟩);
   . assumption;
   . replace eq := Formula.complement.resort_box eq;
     subst eq;
-    trivial;
+    exact hi hq;
 
 class ComplementaryClosed (P : Formulae α) (S : Formulae α) : Prop where
   subset : P ⊆ S⁻
