Logic/Modal/Standard/Kripke/Grz/Completeness.lean
@@ -1,0 +1,282 @@
+import Logic.Modal.Standard.Complemental
+import Logic.Modal.Standard.Kripke.Grz.Definability
+
+
+namespace LO.Modal.Standard
+
+variable {α : Type u} [Inhabited α] [DecidableEq α]
+variable {p q : Formula α}
+
+namespace Formula
+
+noncomputable abbrev GrzSubformulas (p : Formula α) := (𝒮 p) ∪ ((𝒮 p).prebox.image (λ q => □(q ⟶ □q)))
+prefix:70 "𝒮ᴳ " => Formula.GrzSubformulas
+
+namespace GrzSubformulas
+
+@[simp]
+lemma mem_self : p ∈ 𝒮ᴳ p := by simp [GrzSubformulas, Subformulas.mem_self]
+
+lemma mem_boximpbox (h : q ∈ (𝒮 p).prebox) : □(q ⟶ □q) ∈ 𝒮ᴳ p := by simp_all [GrzSubformulas];
+
+lemma mem_origin (h : q ∈ 𝒮 p) : q ∈ 𝒮ᴳ p := by simp_all [GrzSubformulas];
+
+lemma mem_imp (h : (q ⟶ r) ∈ 𝒮ᴳ p) : q ∈ 𝒮ᴳ p ∧ r ∈ 𝒮ᴳ p := by
+  simp_all [GrzSubformulas];
+  aesop;
+
+lemma mem_imp₁ (h : (q ⟶ r) ∈ 𝒮ᴳ p) : q ∈ 𝒮ᴳ p := mem_imp h |>.1
+
+lemma mem_imp₂ (h : (q ⟶ r) ∈ 𝒮ᴳ p) : r ∈ 𝒮ᴳ p := mem_imp h |>.2
+
+macro_rules | `(tactic| trivial) => `(tactic|
+    first
+    | apply mem_origin $ by assumption
+    | apply mem_imp₁  $ by assumption
+    | apply mem_imp₂  $ by assumption
+  )
+
+end GrzSubformulas
+
+
+end Formula
+
+namespace Kripke
+
+open Formula
+
+abbrev GrzCompleteFrame (p : Formula α) : Kripke.FiniteFrame where
+  World := CCF 𝐆𝐫𝐳 (𝒮ᴳ p)
+  Rel X Y :=
+    (∀ q ∈ □''⁻¹(𝒮ᴳ p), □q ∈ X.formulae → □q ∈ Y.formulae) ∧
+    ((∀ q ∈ □''⁻¹(𝒮ᴳ p), □q ∈ Y.formulae → □q ∈ X.formulae) → X = Y)
+
+namespace GrzCompleteFrame
+
+lemma reflexive : Reflexive (GrzCompleteFrame p).Rel := by simp [Reflexive];
+
+lemma transitive : Transitive (GrzCompleteFrame p).Rel := by
+  simp;
+  rintro X Y Z ⟨RXY₁, RXY₂⟩ ⟨RYZ₁, RYZ₂⟩;
+  constructor;
+  . rintro q hq₁ hq₂;
+    exact RYZ₁ q hq₁ $ RXY₁ q hq₁ hq₂;
+  . intro h;
+    have eXY : X = Y := RXY₂ $ by
+      intro q hs hq;
+      exact h q hs $ RYZ₁ q hs hq;
+    have eYZ : Y = Z := RYZ₂ $ by
+      intro q hs hq;
+      exact RXY₁ q hs $ h q hs hq;
+    subst_vars;
+    tauto;
+
+lemma antisymm : Antisymmetric (GrzCompleteFrame p).Rel := by
+  rintro X Y ⟨_, h₁⟩ ⟨h₂, _⟩;
+  exact h₁ h₂;
+
+end GrzCompleteFrame
+
+abbrev GrzCompleteModel (p : Formula α) : Kripke.Model α where
+  Frame := GrzCompleteFrame p
+  Valuation X a := (atom a) ∈ X.formulae
+
+
+open System System.FiniteContext
+open Formula.Kripke
+open ComplementaryClosedConsistentFormulae
+
+
+private lemma Grz_truthlemma.lemma1
+  {X : CCF 𝐆𝐫𝐳 (𝒮ᴳ p)} (hq : □q ∈ 𝒮 p)
+  : ((X.formulae.prebox.box) ∪ {□(q ⟶ □q), -q}) ⊆ (𝒮ᴳ p)⁻ := by
+  simp only [Formulae.complementary];
+  intro r hr;
+  simp [Finset.mem_union] at hr;
+  apply Finset.mem_union.mpr;
+  rcases hr with (rfl | ⟨r, hr, rfl⟩ | rfl);
+  . left;
+    simp;
+    tauto;
+  . have := X.closed.subset hr;
+    left;
+    exact Formulae.complementary_mem_box GrzSubformulas.mem_imp₁ this;
+  . right; simp;
+    use q;
+    constructor;
+    . left; trivial;
+    . rfl;
+
+private lemma Grz_truthlemma.lemma2
+  {X : CCF 𝐆𝐫𝐳 (𝒮ᴳ p)} (hq₁ : □q ∈ 𝒮 p) (hq₂ : □q ∉ X.formulae)
+  : Formulae.Consistent 𝐆𝐫𝐳 ((X.formulae.prebox.box) ∪ {□(q ⟶ □q), -q}) := by
+    apply Formulae.intro_union_consistent;
+    rintro Γ₁ Γ₂ ⟨hΓ₁, hΓ₂⟩;
+    replace hΓ₂ : ∀ r ∈ Γ₂, r = □(q ⟶ □q) ∨ r = -q := by
+      intro r hr;
+      simpa using hΓ₂ r hr;
+
+    by_contra hC;
+    have : Γ₁ ⊢[𝐆𝐫𝐳]! ⋀Γ₂ ⟶ ⊥ := provable_iff.mpr $ and_imply_iff_imply_imply'!.mp hC;
+    have : Γ₁ ⊢[𝐆𝐫𝐳]! (□(q ⟶ □q) ⋏ -q) ⟶ ⊥ := imp_trans''! (by
+      suffices Γ₁ ⊢[𝐆𝐫𝐳]! ⋀[□(q ⟶ □q), -q] ⟶ ⋀Γ₂ by
+        simpa only [ne_eq, List.cons_ne_self, not_false_eq_true, List.conj₂_cons_nonempty, List.conj₂_singleton];
+      apply conjconj_subset!;
+      simpa using hΓ₂;
+    ) this;
+    have : Γ₁ ⊢[𝐆𝐫𝐳]! □(q ⟶ □q) ⟶ -q ⟶ ⊥ := and_imply_iff_imply_imply'!.mp this;
+    have : Γ₁ ⊢[𝐆𝐫𝐳]! □(q ⟶ □q) ⟶ q := by
+      rcases Formula.complement.or (p := q) with (hp | ⟨q, rfl⟩);
+      . rw [hp] at this;
+        exact imp_trans''! this dne!;
+      . simpa only [complement] using this;
+    have : (□'Γ₁) ⊢[𝐆𝐫𝐳]! □(□(q ⟶ □q) ⟶ q) := contextual_nec! this;
+    have : (□'Γ₁) ⊢[𝐆𝐫𝐳]! q := axiomGrz! ⨀ this;
+    have : (□'□'Γ₁) ⊢[𝐆𝐫𝐳]! □q := contextual_nec! this;
+    -- TODO: `contextual_axiomFour`
+    have : 𝐆𝐫𝐳 ⊢! ⋀□'□'Γ₁ ⟶ □q := provable_iff.mp this;
+    have : 𝐆𝐫𝐳 ⊢! □□⋀Γ₁ ⟶ □q := imp_trans''! (imp_trans''! (distribute_multibox_conj! (n := 2)) $ conjconj_subset! (by simp)) this;
+    have : 𝐆𝐫𝐳 ⊢! □⋀Γ₁ ⟶ □q := imp_trans''! axiomFour! this;
+    have : 𝐆𝐫𝐳 ⊢! ⋀□'Γ₁ ⟶ □q := imp_trans''! collect_box_conj! this;
+    have : 𝐆𝐫𝐳 ⊢! ⋀□'(X.formulae.prebox.box |>.toList) ⟶ □q := imp_trans''! (conjconj_subset! (by
+      simp;
+      intro r hr;
+      have := hΓ₁ _ hr; simp at this;
+      tauto;
+    )) this;
+    have : 𝐆𝐫𝐳 ⊢! ⋀□'(X.formulae.prebox.toList) ⟶ □q := imp_trans''! (conjconj_provable! (by
+      intro q hq;
+      simp at hq;
+      obtain ⟨r, hr, rfl⟩ := hq;
+      apply axiomFour'!;
+      apply FiniteContext.by_axm!;
+      simpa;
+    )) this;
+    have : X.formulae *⊢[𝐆𝐫𝐳]! □q := by
+      apply Context.provable_iff.mpr;
+      use □'X.formulae.prebox.toList;
+      constructor;
+      . simp;
+      . assumption;
+    have : □q ∈ X.formulae := membership_iff (by trivial) |>.mpr this;
+    contradiction;
+
+-- TODO: syntactical proof
+private lemma Grz_truthlemma.lemma3 : 𝐊𝐓 ⊢! (p ⋏ □(p ⟶ □p)) ⟶ □p := by
+  by_contra hC;
+  have := (not_imp_not.mpr $ KT_complete (α := α) |>.complete) hC;
+  simp at this;
+  obtain ⟨F, F_refl, hF⟩ := this;
+  simp [ValidOnFrame, ValidOnModel, Satisfies] at hF;
+  obtain ⟨V, x, h₁, h₂, ⟨y, Rxy, h₃⟩⟩ := hF;
+  have := h₂ x (F_refl x);
+  have := (this h₁) _ Rxy;
+  contradiction;
+
+lemma Grz_truthlemma {X : (GrzCompleteModel p).World} (q_sub : q ∈ 𝒮 p) :
+  Satisfies (GrzCompleteModel p) X q ↔ q ∈ X.formulae := by
+  induction q using Formula.rec' generalizing X with
+  | hatom => simp [Satisfies];
+  | hfalsum => simp [Satisfies];
+  | himp q r ihq ihr =>
+    constructor;
+    . contrapose;
+      intro h;
+      simp [Satisfies];
+      constructor;
+      . apply ihq (by trivial) |>.mpr;
+        exact iff_not_mem_imp
+          (hsub_qr := GrzSubformulas.mem_origin q_sub)
+          (hsub_q := by simp [GrzSubformulas]; left; trivial)
+          (hsub_r := by simp [GrzSubformulas]; left; trivial)
+          |>.mp h |>.1;
+      . apply ihr (by trivial) |>.not.mpr;
+        have := iff_not_mem_imp
+          (hsub_qr := GrzSubformulas.mem_origin q_sub)
+          (hsub_q := by simp [GrzSubformulas]; left; trivial)
+          (hsub_r := by simp [GrzSubformulas]; left; trivial)
+          |>.mp h |>.2;
+        exact iff_mem_compl (by simp [GrzSubformulas]; left; trivial) |>.not.mpr (by simpa using this);
+    . contrapose;
+      intro h; simp [Satisfies] at h;
+      obtain ⟨hq, hr⟩ := h;
+      replace hq := ihq (by trivial) |>.mp hq;
+      replace hr := ihr (by trivial) |>.not.mp hr;
+      apply iff_not_mem_imp
+        (hsub_qr := GrzSubformulas.mem_origin q_sub)
+        (hsub_q := by simp [GrzSubformulas]; left; trivial)
+        (hsub_r := by simp [GrzSubformulas]; left; trivial) |>.mpr;
+      constructor;
+      . assumption;
+      . simpa using iff_mem_compl (by simp [GrzSubformulas]; left; trivial) |>.not.mp (by simpa using hr);
+  | hbox q ih =>
+    constructor;
+    . contrapose;
+      by_cases w : q ∈ X.formulae;
+      . intro h;
+        obtain ⟨Y, hY⟩ := lindenbaum (S := 𝒮ᴳ p) (Grz_truthlemma.lemma1 q_sub) (Grz_truthlemma.lemma2 q_sub h);
+        simp only [Finset.union_subset_iff] at hY;
+        simp only [Satisfies]; push_neg;
+        use Y;
+        constructor;
+        . simp [Frame.Rel'];
+          constructor;
+          . intro r hr hr₂;
+            apply hY.1;
+            simpa;
+          . apply imp_iff_not_or (b := X = Y) |>.mpr;
+            left; push_neg;
+            use (q ⟶ □q);
+            refine ⟨?_, ?_, ?_⟩;
+            . right; use q;
+            . apply hY.2; simp;
+            . by_contra hC;
+              have : ↑X.formulae *⊢[𝐆𝐫𝐳]! q := membership_iff (by simp; left; trivial) |>.mp w;
+              have : ↑X.formulae *⊢[𝐆𝐫𝐳]! □(q ⟶ □q) := membership_iff (by simp; right; assumption) |>.mp hC;
+              have : ↑X.formulae *⊢[𝐆𝐫𝐳]! (q ⋏ □(q ⟶ □q)) ⟶ □q := Context.of! $ reducible_KT_Grz Grz_truthlemma.lemma3;
+              have : ↑X.formulae *⊢[𝐆𝐫𝐳]! □q := this ⨀ and₃'! (by assumption) (by assumption);
+              have : □q ∈ X.formulae := membership_iff (GrzSubformulas.mem_origin (by assumption)) |>.mpr this;
+              contradiction;
+        . apply ih (by trivial) |>.not.mpr;
+          apply iff_mem_compl (GrzSubformulas.mem_origin (by trivial)) |>.not.mpr;
+          simp;
+          apply hY.2;
+          simp;
+      . intro _;
+        simp only [Satisfies]; push_neg;
+        use X;
+        constructor;
+        . exact GrzCompleteFrame.reflexive X;
+        . exact ih (by trivial) |>.not.mpr w;
+    . intro h Y RXY;
+      apply ih (by trivial) |>.mpr;
+      have : ↑Y.formulae *⊢[𝐆𝐫𝐳]! □q ⟶ q := Context.of! $ axiomT!;
+      have : ↑Y.formulae *⊢[𝐆𝐫𝐳]! q := this ⨀ (membership_iff (by simp; left; trivial) |>.mp (RXY.1 q (by simp; tauto) h));
+      exact membership_iff (by simp; left; trivial) |>.mpr this;
+
+private lemma Grz_completeAux {p : Formula α} : ReflexiveTransitiveAntisymmetricFrameClass.{u}ꟳ# ⊧ p → 𝐆𝐫𝐳 ⊢! p := by
+  contrapose;
+  intro h;
+  apply exists_finite_frame.mpr;
+  use (GrzCompleteFrame p);
+  constructor;
+  . refine ⟨GrzCompleteFrame.reflexive, GrzCompleteFrame.transitive, GrzCompleteFrame.antisymm⟩;
+  . simp only [ValidOnFrame.models_iff, ValidOnFrame, ValidOnModel.iff_models, ValidOnModel, Satisfies.iff_models];
+    push_neg;
+    obtain ⟨X, hX₁⟩ := lindenbaum (S := 𝒮ᴳ p) (X := {-p})
+      (by simp; apply Formulae.complementary_comp; simp)
+      (Formulae.unprovable_iff_singleton_compl_consistent.mp h);
+    use (GrzCompleteModel p).Valuation, X;
+    apply Grz_truthlemma (by simp) |>.not.mpr;
+    exact iff_mem_compl (by simp) |>.not.mpr $ by
+      simp;
+      apply hX₁;
+      tauto;
+
+instance Grz_complete : Complete (𝐆𝐫𝐳 : DeductionParameter α) ReflexiveTransitiveAntisymmetricFrameClass.{u}ꟳ# := ⟨Grz_completeAux⟩
+
+instance : FiniteFrameProperty (α := α) 𝐆𝐫𝐳 ReflexiveTransitiveAntisymmetricFrameClass where
+
+end Kripke
+
+end LO.Modal.Standard
